Encoding: Attempt to prove more

TM/Encoding.v
@@ -2,79 +2,84 @@ Require Import Prelim LiftNM Compound.
 
 (** * Coding Alphabet *)
 Inductive codsig : Type :=
-| Tup : codsig
 | Con : codsig
 | Nil : codsig
 | Inl : codsig
 | Inr : codsig.
 
 Instance codsig_dec : eq_dec codsig.
-Proof. intros x y. hnf. decide equality. Qed.
+Proof. intros x y. hnf. decide equality. Defined.
 
 (** * Coding Types **)
 
 Inductive codtype : Type :=
-| enctuple : forall (t1 t2 : codtype), codtype
-| enclist  : forall (t : codtype), codtype
-| encsum   : forall (t1 t2 : codtype), codtype
-| encunit  : codtype.
+| codtuple : forall (t1 t2 : codtype), codtype
+| codlist  : forall (t : codtype), codtype
+| codsum   : forall (t1 t2 : codtype), codtype
+| codunit  : codtype.
 
 Instance codtype_dec : eq_dec codsig.
-Proof. intros x y. hnf. decide equality. Qed.
+Proof. intros x y. hnf. decide equality. Defined.
 
 (** Compound Types *)
-Definition encnat := enclist encunit.
-Definition encbool := encsum encunit encunit.
-Definition encopt (t : codtype) := encsum t encunit.
-Definition enctriple (t1 t2 t3 : codtype) := enctuple t1 (enctuple t2 t3).
+Definition codnat := codlist codunit.
+Definition codbool := codsum codunit codunit.
+Definition codopt (t : codtype) := codsum t codunit.
+Definition codtriple (t1 t2 t3 : codtype) := codtuple t1 (codtuple t2 t3).
 
 Fixpoint codtype_to_type (t : codtype) : Type :=
   match t with
-  | enctuple t1 t2 => prod (codtype_to_type t1) (codtype_to_type t2)
-  | enclist  t     => list (codtype_to_type t)
-  | encsum   t1 t2 => sum  (codtype_to_type t1) (codtype_to_type t2)
-  | encunit        => unit
+  | codtuple t1 t2 => prod (codtype_to_type t1) (codtype_to_type t2)
+  | codlist  t     => list (codtype_to_type t)
+  | codsum   t1 t2 => sum  (codtype_to_type t1) (codtype_to_type t2)
+  | codunit        => unit
   end.
 
 
 (** * Encoding *)
-Fixpoint encode_list (t : codtype) (xs : list (codtype_to_type t)) : list codsig.
+
+Definition encoding_function (t : codtype) :=
+  forall v : codtype_to_type t, list codsig.
+
+Fixpoint encode_list (t : codtype) (encode_entries : encoding_function t) (xs : list (codtype_to_type t)) : list codsig.
 Proof.
   destruct xs.
   - apply (Nil :: nil).
-  - apply (cons Con). apply (encode_list t xs).
+  - apply (cons Con). apply app. apply (encode_entries c). apply (encode_list t encode_entries xs).
 Defined.
     
 Fixpoint encode (t : codtype) : codtype_to_type t -> list codsig.
 Proof.
   destruct t; cbn.
-  - intros (a,b). apply (Tup :: encode t1 a ++ encode t2 b).
-  - apply encode_list.
+  - intros (a,b). apply (encode t1 a ++ encode t2 b).
+  - apply encode_list. intros v. apply (encode t v).
   - intros [a|b].
     + apply (Inl :: encode t1 a).
     + apply (Inr :: encode t2 b).
   - intros _. apply nil.
 Defined.
 
+(** * Convert from Coq Type *)
 
-(** * Decoding *)
-
-Ltac invalid_encoding := apply None.
-
-Print codtype.
-
-Inductive decoding_tree : codtype -> list codsig -> Type :=
-| tree_prod (e1 e2 : codtype) (t1 t2 : list codsig) :
-    decoding_tree e1 t1 -> decoding_tree e2 t2 ->
-    decoding_tree (enctuple e1 e2) (Tup :: t1 ++ t2)
-| tree_unit : decoding_tree encunit []
-| tree_invalid (e : codtype) (t : list codsig) : decoding_tree e t.
+Definition from_bool (b : bool) := if b then inl tt else inr tt.
+Definition from_option (t : codtype) (o : option (codtype_to_type t)) :=
+  match o with Some d => inl d | None => inr tt end.
+Fixpoint from_nat n : (codtype_to_type codnat) :=
+  match n with
+  | S n' => tt :: from_nat n'
+  | O => nil
+  end.
 
 
+(** Test *)
+Compute @encode (codtuple (codopt codbool) codnat) (@from_option codbool (Some (from_bool false)), from_nat 3).
+Compute @encode (codtuple (codopt codbool) codnat) (@from_option codbool None, from_nat 3).
 
+
+(** * Suffix *)
 
 Definition suffix (X : Type) (xs ys : list X) :=
-  { n : nat | List.skipn n ys = xs }.
+  exists n : nat, List.skipn n ys = xs.
 
 Lemma suffix_nil (X : Type) (xs : list X) : suffix [] xs.
 Proof.
@@ -106,6 +111,14 @@ Qed.
 Lemma suffix_skip (X : Type) (xs ys : list X) (y : X) :
   suffix xs ys -> suffix xs (y :: ys).
 Proof. intros (n&<-). exists (S n). cbn. reflexivity. Qed.
+
+Lemma suffix_app (X : Type) (xs ys zs : list X) :
+  suffix xs ys -> suffix xs (zs ++ ys).
+Proof.
+  induction zs; intros H.
+  - now rewrite app_nil_l.
+  - cbn. apply suffix_skip. auto.
+Qed.
 
 Lemma suffix_full (X : Type) (xs : list X) :
   suffix xs xs.
@@ -177,37 +190,70 @@ Proof.
 Qed.
 
 
-
 Inductive suffix_induction : list codsig -> Type :=
-| suffix_induction_nil : suffix_induction []
 | suffix_induction_con (ys : list codsig) : (forall xs: list codsig, suffix xs ys -> xs <> ys -> suffix_induction xs) ->
                                             suffix_induction ys.
 
 Inductive size_ind (X : Type) (f : X -> nat) : X -> Type :=
 | size_ind_intro (x : X) : (forall y, f y < f x -> size_ind f y) -> size_ind f x.
 
+
+(* Opaque proofes for size_Ind *)
+Lemma nat_lt_0 (n : nat) : ~n < 0. Proof. omega. Qed.
+Lemma nat_lt_tran_S (a b c : nat) : b < S c -> a < b -> a < c. Proof. omega. Qed.
+
 Lemma size_Ind (X : Type) (f : X -> nat) (x : X) : size_ind f x.
 Proof.
   constructor.
-  assert (G: forall n y, f y < n -> size_ind f y).
-  { intros n. induction n.
-    - intros y B. exfalso. omega.
-    - intros y B. constructor. intros z C. apply IHn. omega. }
-  apply G.
-Qed.
+  generalize (f x) as n.
+  induction n; intros y B.
+  - now apply nat_lt_0 in B.
+  - constructor. intros z C. apply IHn. eapply nat_lt_tran_S; eauto.
+Defined.
 
 Lemma suffix_induction_provider (ys : list codsig) : suffix_induction ys.
 Proof.
-  pose proof (size_Ind (@List.length codsig) ys) as X.
-  induction X as [ys _ IH].
-  destruct ys.
-  - constructor.
-  - constructor. intros xs H1 H2. apply IH. cbn. pose proof (suffix_size_decrease H2 H1). cbn in *. omega.
+  pose proof (size_Ind (@List.length codsig) ys) as X. induction X as [ys _ IH].
+  constructor. intros xs H1 H2. apply IH. now apply (suffix_size_decrease H2 H1).
+Defined.
+
+
+(** * Prefix *)
+
+Definition prefix (X : Type) (xs ys : list X) :=
+  exists n : nat, firstn n ys = xs.
+
+Lemma prefix_full (X : Type) (xs : list X) :
+  prefix xs xs.
+Proof. exists (|xs|). apply List.firstn_all. Qed.
+
+Lemma prefix_app (X : Type) (xs ys zs : list X) :
+  prefix xs ys -> prefix xs (ys ++ zs).
+Proof.
+  intros (n&<-).
+  decide (n < length ys) as [E|E'].
+  - exists (n). rewrite List.firstn_app.
+    replace (n - (| ys |)) with 0 by omega. cbn. rewrite List.app_nil_r. reflexivity.
+  - assert (|ys| <= n) as E by omega.
+    rewrite List.firstn_all2; auto. exists (|ys|). rewrite List.firstn_app.
+    replace ((| ys |) - (| ys |)) with 0 by omega. cbn. rewrite List.app_nil_r. apply List.firstn_all.
 Qed.
 
+Lemma prefix_transitive (X : Type) (xs ys zs : list X) :
+  prefix xs ys -> prefix ys zs -> prefix xs zs.
+Proof. intros (n1&H1) (n2&H2). subst. exists (Nat.min n1 n2). now rewrite List.firstn_firstn. Qed.
+
+
+(** * Decoding *)
+
+Ltac invalid_encoding := apply None.
+
+
+Definition decoding_output (e : codtype) (string : list codsig) :=
+  option (codtype_to_type e * {rest : list codsig & suffix rest string}).
 
 Definition decoding_function (e : codtype) :=
-  forall string : list codsig, option (codtype_to_type e * {rest : list codsig & suffix rest string}).
+  forall string : list codsig, decoding_output e string.
 
 (* TODO: Make this a fixpoint *)
 Definition decode_list' (e : codtype)
@@ -216,58 +262,168 @@ Definition decode_list' (e : codtype)
          (ind : suffix_induction string) :
   option (list (codtype_to_type e) * {rest : list codsig & suffix rest string }).
 Proof.
-  induction ind as [ | string T IH]; cbn in *.
+  induction ind as [string T IH]; cbn in *.
+  destruct string as [ | s ss].
   - invalid_encoding.
-  - destruct string as [ | s ss].
+  - destruct s eqn:E.
+    + (* Con *)
+      destruct (decodeEntries ss) as [ (dec1, (rest1, HRest1)) | ]; [ | invalid_encoding].
+      (* assert (IH : forall xs : list codsig,
+                 suffix xs (Con :: ss) ->
+                 xs <> Con :: ss ->
+                 option
+                   (list (codtype_to_type e) *
+                    {rest : list codsig & suffix rest xs})).
+      {
+        intros ***. apply decode_list'. exact decodeEntries. now apply T.
+      } *)
+      destruct (IH rest1) as [ (dec2, (rest2, HRest2)) | ]; [ | | | invalid_encoding].
+      * now apply suffix_skip.
+      * intros ->. now apply suffix_put in HRest1.
+      * do 2 constructor. apply (dec1 :: dec2). exists rest2. apply suffix_skip. eapply suffix_transitive; eauto.
+    + (* Nil *)
+      do 2 constructor. apply nil. exists ss. apply suffix_skip, suffix_full.
+    + invalid_encoding. + invalid_encoding.
+Defined.
+
+Definition decode_list (e : codtype) (decodeEntries : decoding_function e)
+           (string : list codsig) :=
+  @decode_list' e decodeEntries string (suffix_induction_provider string).
+
+
+Fixpoint decode (t : codtype) (string : list codsig) :
+  option (codtype_to_type t * {rest : list codsig & suffix rest string}).
+Proof.
+  destruct t; cbn in *.
+  - (* tuple *)
+    pose proof (decode t1) as decode1. pose proof (decode t2) as decode2.
+    destruct (decode1 string) as [ (dec1, (rest1, HRest1)) | ]; [ | invalid_encoding].
+    destruct (decode2 rest1)  as [ (dec2, (rest2, Hrest2)) | ]; [ | invalid_encoding].
+    do 2 constructor. constructor. apply dec1. apply dec2. exists rest2. eapply suffix_transitive; eauto.
+  - (* list *)
+    apply (decode_list'). unfold decoding_function. hnf. now apply decode. apply suffix_induction_provider.
+  - (* sum *)
+    pose proof (decode t1) as decode1. pose proof (decode t2) as decode2.
+    destruct string as [ | s ss].
     + invalid_encoding.
     + destruct s eqn:E.
-      * invalid_encoding.
-      * destruct (decodeEntries ss) as [ (dec1, (rest1, HRest1)) | ]; [ | invalid_encoding].
-        (* assert (IH : forall xs : list codsig,
-                   suffix xs (Con :: ss) ->
-                   xs <> Con :: ss ->
-                   option
-                     (list (codtype_to_type e) *
-                      {rest : list codsig & suffix rest xs})).
-        {
-          intros ***. apply decode_list'. exact decodeEntries. now apply T.
-        } *)
-        destruct (IH rest1) as [ (dec2, (rest2, HRest2)) | ]; [ | | | invalid_encoding].
-        -- now apply suffix_skip.
-        -- intros ->. now apply suffix_put in HRest1.
-        -- do 2 constructor. apply (dec1 :: dec2). exists rest2. apply suffix_skip. eapply suffix_transitive; eauto.
-      * invalid_encoding. * invalid_encoding. * invalid_encoding.
-Defined.
-
-
-Fixpoint decode' (Provider : forall (ys : list codsig), suffix_induction ys) (t : codtype)
-         (string : list codsig) : option (codtype_to_type t * {rest : list codsig & suffix rest string}).
-Proof.
-  destruct t eqn:E; cbn in *.
-  - pose proof (decode' Provider c1) as decode1. pose proof (decode' Provider c2) as decode2.
-    destruct string as [ | s ss].
-    + invalid_encoding.
-    + destruct s.
-      * destruct (decode1 ss)    as [ (dec1, (rest1, HRest1)) | ]; [ | invalid_encoding].
-        destruct (decode2 rest1) as [ (dec2, (rest2, Hrest2)) | ]; [ | invalid_encoding].
-        do 2 constructor. constructor. apply dec1. apply dec2. exists rest2. apply suffix_skip. eapply suffix_transitive; eauto.
-      * invalid_encoding. * invalid_encoding. * invalid_encoding. * invalid_encoding.
-  - apply (decode_list'). unfold decoding_function. hnf. now apply (decode' Provider). apply Provider.
-  - pose proof (decode' Provider c1) as decode1. pose proof (decode' Provider c2) as decode2.
-    destruct string as [ | s ss].
-    + invalid_encoding.
-    + destruct s.
-      * invalid_encoding. * invalid_encoding. * invalid_encoding.
-      * destruct (decode1 ss) as [ (dec, (rest, HRest)) | ]; [ | invalid_encoding].
+      * invalid_encoding. * invalid_encoding.
+      * (* Inl *)
+        destruct (decode1 ss) as [ (dec, (rest, HRest)) | ]; [ | invalid_encoding].
         constructor. constructor. left.  apply dec. exists rest. now apply suffix_skip.
-      * destruct (decode2 ss) as [ (dec, (rest, HRest)) | ]; [ | invalid_encoding].
+      * (* Inr *)
+        destruct (decode2 ss) as [ (dec, (rest, HRest)) | ]; [ | invalid_encoding].
         constructor. constructor. right. apply dec. exists rest. now apply suffix_skip.
-  - do 2 constructor. constructor. exists string. apply suffix_full.
+  - (* unit *)
+    do 2 constructor. constructor. exists string. apply suffix_full.
 Defined.
 
-Definition decode (t : codtype) : decoding_function t.
-Proof. intros string. apply decode'. apply suffix_induction_provider. Defined.
 
+(** * Encode and decode *) 
 
+(** Test *)
 
-(** * Encode and decode *)
+Compute decode (codunit) [].
+Compute decode (codtuple codunit codunit) [].
+Compute decode (codtriple codunit codunit codunit) [].
+Compute decode (codtuple (codopt codbool) codnat) (@encode (codtuple (codopt codbool) codnat)
+                                                           (@from_option codbool (Some (from_bool false)), from_nat 3)).
+Compute decode (codtuple (codopt codbool) codnat) (@encode (codtuple (codopt codbool) codnat)
+                                                           (@from_option codbool None, from_nat 3)).
+
+Lemma decode_monoton (t : codtype) (string1 string2 : list codsig) :
+  match decode t (string1) with
+  | Some (v, rest) => match decode t (string1 ++ string2) with
+                     | Some (v', rest') => v = v' /\ prefix (projT1 rest) (projT1 rest')
+                     | None => False
+                     end
+  | None => True
+  end.
+Proof.
+  revert string1 string2. induction t; intros string1 string2; cbn in *.
+  - destruct (decode t1 string1) as [(v1, (rest1, Hrest1))| ] eqn:E1; auto.
+    destruct (decode t1 (string1 ++ string2)) as [(vt, (restt, Hrestt))| ] eqn:E2.
+    + destruct (decode t2 rest1) as [(v2, (rest2, Hrest2))| ] eqn:E3; cbn in *; auto.
+      destruct (decode t2 restt) as [(v2',(rest2',Hrest2'))| ]eqn:E4; cbn in *.
+      * pose proof (IHt1 string1 string2) as IHt1'.
+        rewrite E1 in IHt1'. rewrite E2 in IHt1'. destruct IHt1' as (->&IHt1'). cbn in *.
+        pose proof (IHt2 rest1 rest2') as IHt2'.
+        rewrite E3 in IHt2'. cbn in *.
+        destruct (decode t2 (rest1 ++ rest2')) as [(v3, (rest3, Hrest3))| ] eqn:E5; cbn in *; auto.
+        destruct IHt2' as (->&IHt2'). admit.
+      *
+        specialize (IHt1 string1 string2). rewrite E1 in IHt1. rewrite E2 in IHt1.
+        destruct IHt1 as (->&IHt1).
+        specialize (IHt2 rest1 rest2). rewrite E3 in IHt2.
+        destruct (decode t2 (rest1 ++ rest2)) eqn:E5; cbn in *; auto.
+        destruct p. destruct IHt2 as (->&IHt2).
+        admit.
+    + specialize (IHt1 string1 string2). specialize (IHt2 string1 string2).
+      now erewrite E2, E1 in *.
+  - admit.
+  - destruct string1 eqn:E; auto; cbn in *. destruct c eqn:E2; cbn in *; auto.
+    + destruct (decode t1 l) as [(v1, (rest1, Hrest1))| ] eqn:E3; auto.
+      destruct (decode t1 (l ++ string2)) as [(v2, (rest2, Hrest2))| ] eqn:E4; cbn in *; auto.
+      * specialize (IHt1 l string2). rewrite E3 in IHt1. rewrite E4 in IHt1. destruct IHt1 as (->&IHt1); cbn in *.
+        split; auto.
+      * specialize (IHt1 l string2). rewrite E3 in IHt1. rewrite E4 in IHt1; auto.
+    + destruct (decode t2 l) as [(v1, (rest1, Hrest1))| ] eqn:E3; cbn in *; auto.
+      destruct (decode t2 (l ++ string2)) as [(v2, (rest2, Hrest2))| ] eqn:E4; cbn in *; auto.
+      * specialize (IHt2 l string2). rewrite E3 in IHt2. rewrite E4 in IHt2. destruct IHt2 as (->&IHt2); cbn in *.
+        split; auto.
+      * specialize (IHt2 l string2). rewrite E3 in IHt2. rewrite E4 in IHt2; auto.
+  - split. reflexivity. apply prefix_app, prefix_full.
+Admitted.
+
+Lemma encode_decode_list (t : codtype) (ls : list (codtype_to_type t))
+      (decode_entries : decoding_function t)
+      (encode_entries : encoding_function t) :
+  (forall v : (codtype_to_type t),
+      match decode_entries (encode_entries v) with
+      | Some (v', rest) => v = v' /\ projT1 rest = []
+      | None => False
+      end) ->
+  match decode_list decode_entries (@encode_list t encode_entries ls) with
+  | Some (ls', rest) => ls = ls' /\ projT1 rest = []
+  | None => False
+  end.
+Proof.
+  intros H. unfold decode_list.
+  induction ls as [ | l ls IH].
+  - cbn. auto. (* holds, when you "Defined." instead of "Qed." suffix_induction_provider and size_Ind. *)
+  - cbn.
+    destruct (decode_entries (encode_entries l ++ encode_list encode_entries ls)) as [(vt, (restt, Hrestt))| ] eqn:E1; cbn in *; auto.
+    + destruct restt eqn:E2; cbn in *; auto.
+      * admit.
+      * destruct c eqn:E3; cbn in *; auto. admit. admit. admit. admit.
+    + admit.
+Admitted.
+  
+
+Lemma encode_decode (t : codtype) (v : codtype_to_type t) (string : list codsig) :
+  match decode t (encode v) with
+  | Some (v', rest) => v = v' /\ projT1 rest = []
+  | None => False
+  end.
+Proof.
+  induction t; cbn in *.
+  - destruct v as (v1, v2); cbn in *.
+    destruct (decode t1 (encode v1 ++ encode v2)) as [(dec1, (rest1, HRest1)) | ] eqn:E1; cbn in *.
+    + destruct (decode t2 rest1) as [(dec2, (rest2, HRest2)) | ] eqn:E2; cbn in *.
+      *
+        specialize (IHt2 dec2).
+        destruct (decode t2 (encode dec2)) as [(v2',Rest2')| ] eqn:E3; auto.
+        destruct IHt2 as (->&IHt2).
+        admit.
+      * admit.
+    + admit.
+  - apply encode_decode_list. auto.
+  - destruct v as [v|v].
+    + destruct (decode t1 (encode v)) as [(v1, (rest1, Hrest1))| ] eqn:E; cbn in *; auto.
+      * specialize (IHt1 v). rewrite E in IHt1. cbn in *. intuition; subst; auto.
+      * specialize (IHt1 v). rewrite E in IHt1. cbn in *. intuition; subst; auto.
+    + destruct (decode t2 (encode v)) as [(v2, (rest2, Hrest2))| ] eqn:E; cbn in *; auto.
+      * specialize (IHt2 v). rewrite E in IHt2. cbn in *. intuition; subst; auto.
+      * specialize (IHt2 v). rewrite E in IHt2. cbn in *. intuition; subst; auto.
+  - destruct v. auto.
+Admitted.
